tests/lean/case.lean
@@ -1,0 +1,34 @@
+example (xs : list ℕ) : ℕ :=
+begin
+  induction xs,
+  case list.cons {}
+end
+
+example (xs : list ℕ) : ℕ :=
+begin
+  cases xs,
+  case list.cons {}
+end
+
+example (xs : list ℕ) : ℕ :=
+begin
+  induction xs,
+  case list.cons x xs {
+    cases xs,
+    case list.cons x xs {}
+  }
+end
+
+open list
+example (xs : list ℕ) : ℕ :=
+begin
+  induction xs,
+  case cons {}
+end
+
+example (xs : list ℕ) : ℕ :=
+begin
+  induction xs,
+  case list.cons x xs ih { apply ih },
+  case list.nil { apply 0 }
+end
